contracts/verification/easycrypt/c10-port/scratch/C10CoverageSinglePath.ec
@@ -1,0 +1,6 @@
+require import AllCore List IntDiv C10HypertreeCoverage.
+lemma one_path_covers_cell :
+  (forall layer, 0 <= layer < 2 =>
+    !(layer = 0 /\ (path_cell 0 layer).`1 = 1 /\ (path_cell 0 layer).`2 = 0)) =>
+  !(0 = 0 /\ 1 = 1 /\ 0 = 0).
+proof. by rewrite /path_cell subtree_width /=. qed.
