contracts/verification/easycrypt/c10-port/scratch/C10RandomizerWrongHalf.ec
@@ -1,0 +1,3 @@
+require import AllCore List C10Randomizer.
+lemma wrong_half : truncate_r (nseq 128 false ++ nseq 128 true) = nseq 128 false.
+proof. by rewrite /truncate_r drop_cat size_nseq /= drop0. qed.
